Solve the following differential equation:
\[
x\frac{dy}{dx} + (1-y^2) = 0; \quad \quad y = 0 \text{ when } x = 1.
\]
\newline
\[
x\frac{dy}{dx}+ (1-y^2) = 0; (1,0)
\]
\[
x\frac{dy}{dx} = y^2 - 1
\]
\[
\int \frac{1}{x}dx = \int \frac{1}{y^2-1}dy
\]
\[
\int \frac{1}{x}dx = \frac{1}{2}\int \frac{1}{y-1}dy - \frac{1}{2}\int\frac{1}{y+1}dy
\]
\[
\ln x + C =  \frac{1}{2}\ln|y-1| - \frac{1}{2}\ln|y+1|
\]
\[
Cx = \sqrt{\frac{|y-1|}{|y+1|}}.
\]
When $x = 1$, $y = 0$. So
\[
C = \sqrt{\frac{1}{1}} = 1.
\]
\[
C = 1.
\]
\[
x = \sqrt{\frac{|y-1|}{|y+1|}}.
\]
\[
x^2 = \frac{|y-1|}{|y+1|}
\]
\[
x^2y + x^2 = y - 1
\]
\[
x^2 + 1 = y - x^2y
\]
\[
y = \frac{1+x^2}{1-x^2}.
\]