Evaluate the following definite integrals:
\begin{enumerate}
\item $\int^L_0 xe^{-x} \text{ }dx$
\item $\int^{\pi/2}_0 \sin3\theta \cos\theta \text{ }d\theta$
\item $\int^1_0 \dfrac{x^2+1}{x^3+3x+2}\text{ d}x$
\item $\int^{\pi/2}_0 \dfrac{1}{3+5\cos\theta} \text{ }d\theta$ [use $t = \tan(\frac{1}{2}\theta)$].
\end{enumerate}
In part 1, can you suggest what happens as $L \to \infty$.
\begin{enumerate}
\item
First we define
\[
I(L) = \int^L_0 xe^{-x} dx.
\]
Then, by parts, let $u = x$ and $v' = e^{-x}$ so $u' = 1$ and $v = -e^{-x}$ and
\[
I(L) = -xe^{-x}\rvert^L_0 + \int^L_0 e^{-x} dx 	
\]
\[
= (-xe^{-x})\rvert^L_0 + (-e^{-x})\rvert^L_0
\]
\[
= -Le^{-L} - e^{-L} +1
\]
\[
-e^{-L}(L+1) + 1.
\]
As $L \to \infty$, $I(L) \to 1$.
\item
First we define
\[
I = \int^{\pi/2}_0 \sin3\theta\cos\theta d\theta.
\]
Then, by parts, let $u = \sin 3\theta$ and $v' = \cos\theta$ so $u' = 3\cos3\theta$ and $v = \sin\theta$. Then
\[
I = (\sin\theta\sin3\theta)\rvert^{\pi/2}_0 - 3\int \sin\theta\cos3\theta d\theta.
\]
Now, by parts, let $x = \cos 3\theta$ and $y' = \sin \theta$ so that $x' = -3\sin3\theta$ and $y = -\cos\theta$. Then
\[
I = (\sin\theta\sin3\theta)\rvert^{\pi/2}_0 -3(-\cos\theta\cos3\theta - 3\int^{\pi/2}_0 \cos\theta\sin3\theta d\theta)
\]
\[
I = (\sin\theta\sin3\theta)\rvert^{\pi/2}_0 + (3\cos\theta\cos3\theta)\rvert^{\pi/2}_0 + 9I
\]
\[
-8I = (\sin\theta\sin3\theta)\rvert^{\pi/2}_0 + (3\cos\theta\cos3\theta)\rvert^{\pi/2}_0
\]
\[
= (-1 + 0) - (0 + 3)
\]
\[
= -4.
\]
\[
I = \frac{1}{2}.
\]
\item
First we define
\[
I = \int^1_0 \frac{x^2+1}{x^3+3x+2} dx.
\]
Let $u = x^3 + 3x+ 2$ so that $du = dx(3x^2 + 3)$.
Then 
\[
I = \int^6_2 \frac{x^2+1}{u(3x^2+3)} du 
\]
\[
= \int^6_2 \frac{1}{3u}du
\]
\[
= (\frac{1}{3}\ln u)\rvert^6_2
\]
\[
= \frac{1}{3}\ln3.
\]
\item
First we define
\[
I = \int^{\pi/2}_0 \frac{1}{3+5\cos\theta}\text{ }d\theta.
\]
Then we use the standard $t$-substitution. That is, $t = \tan(\frac{1}{2}\theta)$ so $d\theta = \cos^2(\frac{1}{2}\theta)dt$. This gives us
\[
I = \int^1_0 \frac{1}{3 + \frac{5-5t^2}{1+t^2}}\cdot\frac{2}{1+t^2}\text{ }dt
\]
\[
= \int^1_0 \frac{2}{3+3t^2 + 5 - 5t^2}\text{ }dt
\]
\[
= \int^1_0 \frac{2}{8-2t^2}\text{ }dt
\]
\[
=\int^1_0 \frac{1}{4-t^2}\text{ }dt
\]
\[
=\frac{1}{4}\int^1_0 \frac{1}{2+t}\text{ dt} + \frac{1}{4}\int^1_0 \frac{1}{(2-t)}\text{ }dt
\]
\[
=\frac{1}{4}\left(\ln3\right).
\]
\end{enumerate}