State the definitions of sinh $x$ and cosh $x$. Prove that
\[
\text{cosh}^2x - \text{sinh}^2x = 1 \quad \quad \quad \text{sinh}2x = 2 \text{sinh}x\text{cosh}x
\]
\newline
$\sinh x$ is the odd part of the exponential function and $\cosh x$ is the even part. We thus have
\[
\sinh x = \frac{e^x-e^{-x}}{2}
\]
\[
\cosh x = \frac{e^x + e^{-x}}{2}.
\]
A simplie computation reveals
\[
\cosh^2x - \sinh^2x = (\cosh x - \sinh x)(\cosh x + \sinh x)
\]
\[
e^{-x}e^x = 1.
\]
Similarly,
\[
2\sinh x\cosh x = 2\left(\frac{e^x+e^{-x}}{2}\right)\left(\frac{e^x-e^{-x}}{2}\right) 
\]
\[
= \frac{(e^x+e^{-x})(e^x -e^{-x})}{2}
\]
\[
= \frac{e^{2x} -e^{-2x}}{2} = \sinh 2x.
\]