Prove that
\[
\frac{d}{dx}\text{tanh}x = \text{sech}^2x.
\]
\newline
\[
\tanh x = \frac{\sinh x}{\cosh x}
\]
\[
= \frac{e^x -e^{-x}}{e^x+e^{-x}}.
\]
\[
\frac{d}{dx}\tanh x = \frac{d}{dx}(e^x-e^{-x})(e^x+e^{-x})^{-1}
\]
\[
= (e^x +e^{-x})(e^x+e^{-x})^{-1} + (e^x-e^{-x})-1(e^x +e^{-x})^{-2}(e^{x} -e^{-x})
\]
\[
=\frac{e^x + e^{-x}}{e^x + e^{-x}} - \frac{(e^x-e^{-x})(e^x-e^{-x})}{(e^x+e^{-x})^2}
\]
\[
=\frac{(e^x+e^{-x})^2 -(e^x-e^{-x})^2}{(e^x+e^{-x})^2}
\]
\[
= \frac{[(e^x + e^{-x}) + (e^x-e^{-x})][(e^x+e^{-x})-(e^x-e^{-x})]}{(e^x+e^{-x})^2}
\]
\[
= \frac{(2e^x)(2e^{-x})}{(e^x+e^{-x})^2}
\]
\[
= \frac{4}{(e^{x}+e^{-x})^2}
\]
\[
= \frac{1}{(\frac{e^x+e^{-x}}{2})^2}
\]
\[
= \frac{1}{\cosh^2x}
\]
\[
= \text{sech}^2x.
\]