\begin{enumerate}
\item
Divide $x^3 + 5x^2 -2x -24$ by $(x+4)$ and hence factorise it completely.
\[
x^3 + 5x^2 -2x - 24 = (x+4)(x^2+x -6) = (x+4)(x-2)(x+3).
\]
\item
Use the factor theorem to factorise $t^3 - 7t + 6$.
\newline
We note that $(1)^3 -7(1)+6 = 0$ and so by the factor theorem $(t-1)$ is a factor. Then dividing reveals
\[
t^3 - 7t + 6 = (t-1)(t^2+t -6) = (t-1)(t+3)(t-2).
\]
\item
Simplify $\dfrac{x^3+x^2-2x}{x^3+2x^2-x-2}$.
\newline
\newline
We see that $(x-1)$ is a factor of both the numerator and denominator and proceed from there
\[
\frac{x^3+x^2-2x}{x^3+2x^2-x-2} = \frac{\left(x-1\right)\left(x^2+2x\right)}{\left(x-1\right)\left(x^2+3x+2\right)}
\]
\[
= \frac{(x)(x+2)}{(x+2)(x+1)}
\]
\[
=\frac{x}{x+1}.
\]
\end{enumerate}