\begin{enumerate}
\item
\[
\frac{2}{(x+1)(x-1)} = \frac{A}{x+1} + \frac{B}{x-1}.
\]
So we see
\[
2 = Ax - A + Bx + B.
\]
So
\[
A + B = 0 \iff A = -B.
\]
\[
B-A = 2B = 2. 
\]
So $A= -1$, $B=1$.
Thus
\[
\frac{2}{(x+1)(x-1)} = \frac{1}{x-1} - \frac{1}{x+1}.
\]
\item
\[
\frac{x+13}{(x+1)(x-2)(x+3)} = \frac{A}{x+1} + \frac{B}{x-2} + \frac{C}{x+3}.
\]
So
\[
Ax^2 +Ax - 6A + Bx^2 + 4Bx + 3B + Cx^2 -Cx -2C.
\]
\[
A + B + C = 0.
\]
\[
A + 4B - C = 1.
\]
\[
-6A+3B-2C =13. 
\]
Gaussian elimination yields
\[
2A + 5B = 1.
\]
\[
8A + 5B = -11.
\]
So $6A = -12$, so $A = -2$. Hence $B = 1$ and $C = 1$ so
\[
\frac{x+13}{(x+1)(x-2)(x+3)} = \frac{1}{x-2} + \frac{1}{x+3} - \frac{2}{x+1}.
\]
\item
\[
\frac{4x+1}{(x+1)^2(x-2)} = \frac{Ax + B}{(x+1)^2} + \frac{C}{x-2}.
\]
So 
\[
Ax^2 + (B-2A)x -2B + Cx^2 + 2Cx + C = 4x+1.
\]
\[
A + C= 0.
\]
\[
-2A + B + 2C= 4.
\]
\[
-2B + C = 1.
\]
Subbing in $A = -C$,
\[
B + 4C = 4.
\]
\[
-2B + C = 1.
\]
So $9C = 9$, so $C=1$ so $B = 0$ and $A = -1$. Hence
\[
\frac{4x+1}{(x+1)^2(x-2)} = \frac{1}{x-2} - \frac{x}{(x+1)^2}.
\]
\end{enumerate}