If $A, B$ and $C$ are the angles of a triangle, prove that
\[
\cos \left(\frac{B-C}{2} \right)-\sin\left(\frac{A}{2}\right) = 2 \sin\left(\frac{B}{2}\right)\sin\left(\frac{C}{2}\right).
\]
\newline
We first apply a compound angle identity backwards to to the right hand side to obtain
\[
2\sin\left(\frac{B}{2}\right)\sin\left(\frac{C}{2}\right) = \cos\left(\frac{B-C}{2}\right) - \cos\left(\frac{B+C}{2}\right).
\]
Since $A,B$ and $C$ are three internal angles in a triangle we know that $A+B+C = \pi$ and consequently $B+C = \pi - A$, which, when substituted gives us
\[
2\sin\left(\frac{B}{2}\right)\sin\left(\frac{C}{2}\right) = \cos\left(\frac{B-C}{2}\right) - \cos\left(\frac{\pi-A}{2}\right).
\]
But, $\cos\left(\frac{\pi}{2}-\theta\right) = \sin \theta$ and so $\cos\left(\frac{\pi-A}{2}\right) = \sin\left(\frac{A}{2}\right)$, which when substituted gives us, as desired,
\[
2\sin\left(\frac{B}{2}\right)\sin\left(\frac{C}{2}\right) = \cos \left(\frac{B-C}{2} \right)-\sin\left(\frac{A}{2}\right).
\]