Prove that $\dfrac{\cot^2x+\sin^2x}{\cos x + \text{cosec } x} = \text{cosec } x - \cos x$.
\newline
We start by multiplying the right hand side by a carefully chosen form of 1 and proceed from there:
\[
(\text{cosec } x - \cos x)\frac{\text{cosec } x + \cos x}{\text{cosec } x + \cos x}
\]
\[
= \frac{\frac{1}{\sin^2x}-\cos^2x}{\text{cosec }x+ \cos x}
\]
\[
= \frac{\frac{1}{\sin^2x}-(1-\sin^2x)}{\text{cosec }x + \cos x }
\]
\[
= \frac{\frac{1-\sin^2x}{\sin^2x}+\sin^2x}{\text{cosec }x + \cos x}
\]
\[
= \frac{\cot^2x + \sin^2x}{\text{cosec }x + \cos x}.
\]