By writing $\dfrac{\pi}{12} = \dfrac{\pi}{3}- \dfrac{\pi}{4}$, use trigonometric identities to evaluate:
\begin{enumerate}
\item
$\cos \dfrac{\pi}{12}$
\item
$\sin \dfrac{\pi}{12}$
\item
$\cot \dfrac{\pi}{12}$
\end{enumerate}
\begin{enumerate}
\item
\[
\cos\frac{\pi}{12} = \cos\left(\frac{\pi}{3}-\frac{\pi}{4}\right)
\]
\[
=\cos\frac{\pi}{3}\cos\frac{\pi}{4}+\sin\frac{\pi}{3}\sin\frac{\pi}{4}
\]
\[
= \frac{1}{2}\cdot\frac{\sqrt{2}}{2}+\frac{\sqrt{3}}{2}\cdot\frac{\sqrt{2}}{2}
\]
\[
=\frac{\sqrt{6}+\sqrt{2}}{4}.
\]
\item
\[
\sin\frac{\pi}{12} = \sin\left(\frac{\pi}{3}-\frac{\pi}{4}\right)
\]
\[
=\sin\frac{\pi}{3}\cos\frac{\pi}{4} - \sin\frac{\pi}{4}\cos\frac{\pi}{3}
\]
\[
=\frac{\sqrt{3}}{2}\cdot\frac{\sqrt{2}}{2}-\frac{\sqrt{2}}{2}\cdot\frac{1}{2}
\]
\[
= \frac{\sqrt{6}-\sqrt{2}}{4}.
\]
\item
\[
\cot\frac{\pi}{12} = \frac{\cos\frac{\pi}{12}}{\sin\frac{\pi}{12}}
\]
\[
= \frac{\sqrt{6}+\sqrt{2}}{\sqrt{6}-\sqrt{2}}
\]
\[
= \frac{8+4\sqrt{3}}{4}
\]
\[
= 2 + \sqrt{3}.
\]
\end{enumerate}